Fix compilation

misc.v
@@ -49,171 +49,6 @@ Section excl.
   Qed.
 End excl.
 
-Section pair.
-  Context `{EqDecision A, !inG Σ (prodR fracR (dec_agreeR A))}.
-  
-  Lemma m_frag_agree γm (q1 q2: Qp) (a1 a2: A):
-    own γm (q1, DecAgree a1) ★ own γm (q2, DecAgree a2)
-    ⊢ |=r=> own γm ((q1 + q2)%Qp, DecAgree a1) ★ (a1 = a2).
-  Proof.
-    iIntros "[Ho Ho']".
-    destruct (decide (a1 = a2)) as [->|Hneq].
-    - iSplitL=>//.
-      iCombine "Ho" "Ho'" as "Ho".
-      iDestruct (own_update with "Ho") as "?"; last by iAssumption.
-      by rewrite pair_op frac_op' dec_agree_idemp.
-    - iCombine "Ho" "Ho'" as "Ho".
-      iDestruct (own_valid with "Ho") as %Hvalid.
-      exfalso. destruct Hvalid as [_ Hvalid].
-      simpl in Hvalid. apply dec_agree_op_inv in Hvalid. inversion Hvalid. subst. auto.
-  Qed.
-End pair.
-
-Section evidence.  
-  Context (K A: Type) `{Countable K, EqDecision A}.
-  Definition evkR := prodR fracR (dec_agreeR A).
-  Definition evmapR := gmapUR K evkR.
-  Definition evidenceR := authR evmapR.
-  Class evidenceG Σ := EvidenceG { evidence_G :> inG Σ evidenceR }.
-  Definition evidenceΣ : gFunctors := #[ GFunctor (constRF evidenceR) ].
-
-  Instance subG_evidenceΣ {Σ} : subG evidenceΣ Σ → evidenceG Σ.
-  Proof. intros [?%subG_inG _]%subG_inv. split; apply _. Qed.
-
-  Lemma map_agree_eq m m' (hd: K) (p q: Qp) (x y: A):
-    m !! hd = Some (p, DecAgree y) →
-    m = {[hd := (q, DecAgree x)]} ⋅ m' → x = y.
-  Proof.
-    intros H1 H2.
-    destruct (decide (x = y)) as [->|Hneq]=>//.
-    exfalso.
-    subst. rewrite lookup_op lookup_singleton in H1.
-    destruct (m' !! hd) as [[b [c|]]|] eqn:Heqn; rewrite Heqn in H1; inversion H1=>//.
-    destruct (decide (x = c)) as [->|Hneq3]=>//.
-    - rewrite dec_agree_idemp in H3. by inversion H3.
-    - rewrite dec_agree_ne in H3=>//.
-  Qed.
-
-  Lemma map_agree_somebot m m' (hd: K) (p q: Qp) (x: A):
-    m !! hd = Some (p, DecAgreeBot) → m' !! hd = None →
-    m = {[hd := (q, DecAgree x)]} ⋅ m' → False.
-  Proof.
-    intros H1 H2 H3. subst. rewrite lookup_op lookup_singleton in H1.
-    destruct (m' !! hd) as [[b [c|]]|] eqn:Heqn; rewrite Heqn in H1; inversion H1=>//.
-  Qed.
-
-  Lemma map_agree_none m m' (hd: K) (q: Qp) (x: A):
-    m !! hd = None → m = {[hd := (q, DecAgree x)]} ⋅ m' → False.
-  Proof.
-    intros H1 H2. subst. rewrite lookup_op lookup_singleton in H1.
-    destruct (m' !! hd)=>//.
-  Qed.
-
-  Context `{!inG Σ (authR evmapR)}.
-
-  Definition ev γm (k : K) (v: A) := (∃ q, own γm (◯ {[ k := (q, DecAgree v) ]}))%I.
-
-  Lemma evmap_alloc γm m k v:
-    m !! k = None →
-    own γm (● m) ⊢ |=r=> own γm (● (<[ k := (1%Qp, DecAgree v) ]> m) ⋅ ◯ {[ k := (1%Qp, DecAgree v) ]}).
-  Proof.
-    iIntros (?) "Hm".
-    iDestruct (own_update with "Hm") as "?"; last by iAssumption.
-    apply auth_update_alloc, alloc_local_update=>//.
-  Qed.
-  
-  Lemma map_agree_none' γm m hd x:
-    m !! hd = None →
-    own γm (● m) ★ ev γm hd x ⊢ False.
-  Proof.
-    iIntros (?) "[Hom Hev]". iDestruct "Hev" as (?) "Hfrag".
-    iCombine "Hom" "Hfrag" as "Hauth".
-    iDestruct (own_valid γm (● m ⋅ ◯ {[hd := (_, DecAgree x)]})
-               with "[Hauth]") as %Hvalid=>//.
-    iPureIntro.
-    apply auth_valid_discrete_2 in Hvalid as [[af Compose%leibniz_equiv_iff] Valid].
-    eapply (map_agree_none m)=>//.
-  Qed.
-  
-  Lemma map_agree_eq' γm m hd p x agy:
-    m !! hd = Some (p, agy) →
-    own γm (● m) ★ ev γm hd x ⊢ own γm (● m) ★ ev γm hd x ★ DecAgree x = agy.
-  Proof.
-    iIntros (?) "[Hom Hev]". iDestruct "Hev" as (?) "Hfrag".
-    iCombine "Hom" "Hfrag" as "Hauth".
-    iDestruct (own_valid γm (● m ⋅ ◯ {[hd := (_, DecAgree x)]})
-               with "[Hauth]") as %Hvalid=>//.
-    apply auth_valid_discrete_2 in Hvalid as [[af Compose%leibniz_equiv_iff] Valid].
-    destruct agy as [y|].
-    - iDestruct "Hauth" as "[? ?]". iFrame. iSplitL.
-      { rewrite /ev. eauto. }
-      iPureIntro. destruct (decide (x = y)); try by subst.
-      exfalso. apply n. eapply (map_agree_eq m)=>//. (* XXX: Why it is uPred M *)
-    - iAssert (✓ m)%I as "H"=>//. rewrite (gmap_validI m).
-      iDestruct ("H" $! hd) as "%".
-      exfalso. subst. rewrite H0 in H2.
-      by destruct H2 as [? ?].
-  Qed.
-
-  Lemma pack_ev γm k v q:
-    own γm (◯ {[ k := (q, DecAgree v) ]}) ⊢ ev γm k v.
-  Proof. iIntros "?". rewrite /ev. eauto. Qed.
-  
-  Lemma dup_ev γm hd y:
-    ev γm hd y ⊢ |=r=> ev γm hd y ★ ev γm hd y.
-  Proof.
-    rewrite /ev. iIntros "Hev". iDestruct "Hev" as (q) "Hev".
-    iAssert (|=r=> own γm (◯ {[hd := ((q/2)%Qp, DecAgree y)]} ⋅
-                           ◯ {[hd := ((q/2)%Qp, DecAgree y)]}))%I with "[Hev]" as "==>[Hev1 Hev2]".
-    { iDestruct (own_update with "Hev") as "?"; last by iAssumption.
-      rewrite <- auth_frag_op.
-      by rewrite op_singleton pair_op dec_agree_idemp  frac_op' Qp_div_2. }
-    iSplitL "Hev1"; eauto.
-  Qed.
-
-  Lemma evmap_frag_agree_split γm p q1 q2 (a1 a2: A):
-    own γm (◯ {[p := (q1, DecAgree a1)]}) ★
-    own γm (◯ {[p := (q2, DecAgree a2)]})
-    ⊢ |=r=> own γm (◯ {[p := (q1, DecAgree a1)]}) ★
-            own γm (◯ {[p := (q2, DecAgree a1)]}) ★ (a1 = a2).
-  Proof.
-    iIntros "[Ho Ho']".
-    destruct (decide (a1 = a2)) as [->|Hneq].
-    - by iFrame.
-    - iCombine "Ho" "Ho'" as "Ho".
-      iDestruct (own_valid with "Ho") as %Hvalid.
-      exfalso. rewrite <-(@auth_frag_op evmapR) in Hvalid.
-      rewrite op_singleton in Hvalid.
-      apply auth_valid_discrete in Hvalid. simpl in Hvalid.
-      apply singleton_valid in Hvalid.
-      destruct Hvalid as [_ Hvalid].
-      apply dec_agree_op_inv in Hvalid. inversion Hvalid. subst. auto.
-  Qed.
-
-  Lemma evmap_frag_agree γm p q1 q2 (a1 a2: A):
-    own γm (◯ {[p := (q1, DecAgree a1)]}) ★
-    own γm (◯ {[p := (q2, DecAgree a2)]})
-    ⊢ |=r=> own γm (◯ {[p := ((q1 + q2)%Qp, DecAgree a1)]}) ★ (a1 = a2).
-  Proof.
-    iIntros "Hos".
-    iDestruct (evmap_frag_agree_split with "Hos") as "==>[Ho1 [Ho2 %]]".
-    iCombine "Ho1" "Ho2" as "Ho". iSplitL; auto.
-    iDestruct (own_update with "Ho") as "?"; last by iAssumption.
-    rewrite <-(@auth_frag_op evmapR {[p := (q1, DecAgree a1)]} {[p := (q2, DecAgree a1)]}).
-    by rewrite op_singleton pair_op frac_op' dec_agree_idemp.
-  Qed.
-
-  Lemma ev_agree γm k v1 v2:
-    ev γm k v1 ★ ev γm k v2 ⊢ |=r=> ev γm k v1 ★ ev γm k v1 ★ v1 = v2.
-  Proof.
-    iIntros "[Hev1 Hev2]".
-    iDestruct "Hev1" as (?) "Hev1". iDestruct "Hev2" as (?) "Hev2".
-    iDestruct (evmap_frag_agree_split with "[-]") as "==>[Hev1 [Hev2 %]]"; first iFrame.
-    subst. iSplitL "Hev1"; rewrite /ev; eauto.
-  Qed.
-
-End evidence.
-
 Section heap_extra.
   Context `{heapG Σ}.
 
@@ -246,3 +81,23 @@ Section big_op_later.
     ▷ ([★ map] k↦y ∈ <[i:=x]> m, Φ k y) ⊣⊢ ▷ Φ i x ★ ▷ [★ map] k↦y ∈ m, Φ k y.
   Proof. intros ?. rewrite big_sepM_insert=>//. apply later_sep. Qed.
 End big_op_later.
+
+Section pair.
+  Context `{EqDecision A, !inG Σ (prodR fracR (dec_agreeR A))}.
+  
+  Lemma m_frag_agree γm (q1 q2: Qp) (a1 a2: A):
+    own γm (q1, DecAgree a1) ★ own γm (q2, DecAgree a2)
+    ⊢ |=r=> own γm ((q1 + q2)%Qp, DecAgree a1) ★ (a1 = a2).
+  Proof.
+    iIntros "[Ho Ho']".
+    destruct (decide (a1 = a2)) as [->|Hneq].
+    - iSplitL=>//.
+      iCombine "Ho" "Ho'" as "Ho".
+      iDestruct (own_update with "Ho") as "?"; last by iAssumption.
+      by rewrite pair_op frac_op' dec_agree_idemp.
+    - iCombine "Ho" "Ho'" as "Ho".
+      iDestruct (own_valid with "Ho") as %Hvalid.
+      exfalso. destruct Hvalid as [_ Hvalid].
+      simpl in Hvalid. apply dec_agree_op_inv in Hvalid. inversion Hvalid. subst. auto.
+  Qed.
+End pair.
