evmap.v
@@ -1,0 +1,114 @@
+(* evmap.v -- generalized heap-like monoid *)
+From iris.program_logic Require Export invariants weakestpre.
+From iris.algebra Require Export auth frac gmap dec_agree.
+From iris.proofmode Require Import tactics.
+
+Section evmap.
+  Context (K A: Type) (Q: cmraT) `{Countable K, EqDecision A(* , CMRADiscrete Q *)}.
+  Definition evkR := prodR Q (dec_agreeR A).
+  Definition evmapR := gmapUR K evkR.
+  Definition evidenceR := authR evmapR.
+  Class evidenceG Σ := EvidenceG { evidence_G :> inG Σ evidenceR }.
+  Definition evidenceΣ : gFunctors := #[ GFunctor (constRF evidenceR) ].
+
+  Instance subG_evidenceΣ {Σ} : subG evidenceΣ Σ → evidenceG Σ.
+  Proof. intros [?%subG_inG _]%subG_inv. split; apply _. Qed.
+
+  Lemma map_agree_eq m m' (hd: K) (p q: Q) (x y: A):
+    m !! hd = Some (p, DecAgree y) →
+    m = {[hd := (q, DecAgree x)]} ⋅ m' → x = y.
+  Proof.
+    intros H1 H2.
+    destruct (decide (x = y)) as [->|Hneq]=>//.
+    exfalso.
+    subst. rewrite lookup_op lookup_singleton in H1.
+    destruct (m' !! hd) as [[b [c|]]|] eqn:Heqn; rewrite Heqn in H1; inversion H1=>//.
+    destruct (decide (x = c)) as [->|Hneq3]=>//.
+    - rewrite dec_agree_idemp in H3. by inversion H3.
+    - rewrite dec_agree_ne in H3=>//.
+  Qed.
+
+  Lemma map_agree_somebot m m' (hd: K) (p q: Q) (x: A):
+    m !! hd = Some (p, DecAgreeBot) → m' !! hd = None →
+    m = {[hd := (q, DecAgree x)]} ⋅ m' → False.
+  Proof.
+    intros H1 H2 H3. subst. rewrite lookup_op lookup_singleton in H1.
+    destruct (m' !! hd) as [[b [c|]]|] eqn:Heqn; rewrite Heqn in H1; inversion H1=>//.
+  Qed.
+
+  Lemma map_agree_none m m' (hd: K) (q: Q) (x: A):
+    m !! hd = None → m = {[hd := (q, DecAgree x)]} ⋅ m' → False.
+  Proof.
+    intros H1 H2. subst. rewrite lookup_op lookup_singleton in H1.
+    destruct (m' !! hd)=>//.
+  Qed.
+End evmap.
+
+Section evmapR.
+  Context (K A: Type) `{Countable K, EqDecision A}.
+  Context `{!inG Σ (authR (evmapR K A unitR))}.
+
+  Definition ev γm (k : K) (v: A) := own γm (◯ {[ k := ((), DecAgree v) ]})%I.
+
+  Global Instance persistent_ev γm k v : PersistentP (ev γm k v).
+  Proof. apply _. Qed.
+
+  Lemma evmap_alloc γm m k v q:
+    m !! k = None → ✓ q →
+    own γm (● m) ⊢ |=r=> own γm (● (<[ k := (q, DecAgree v) ]> m) ⋅ ◯ {[ k := (q, DecAgree v) ]}).
+  Proof.
+    iIntros (??) "Hm".
+    iDestruct (own_update with "Hm") as "?"; last by iAssumption.
+    apply auth_update_alloc. apply alloc_singleton_local_update=>//.
+  Qed.
+  
+  Lemma map_agree_none' γm (m: evmapR K A unitR) hd x:
+    m !! hd = None →
+    own γm (● m) ★ ev γm hd x ⊢ False.
+  Proof.
+    iIntros (?) "[Hom Hev]".
+    iCombine "Hom" "Hev" as "Hauth".
+    iDestruct (own_valid with "Hauth") as %Hvalid. iPureIntro.
+    apply auth_valid_discrete_2 in Hvalid as [[af Compose%leibniz_equiv_iff] Valid].
+    eapply (map_agree_none _ _ _ m)=>//.
+  Qed.
+
+  Lemma map_agree_eq' γm m hd p x agy:
+    m !! hd = Some (p, agy) →
+    ev γm hd x ★ own γm (● m) ⊢ DecAgree x = agy.
+  Proof.
+    iIntros (?) "[#Hev Hom]".
+    iCombine "Hom" "Hev" as "Hauth".
+    iDestruct (own_valid γm (● m ⋅ ◯ {[hd := (_, DecAgree x)]})
+               with "[Hauth]") as %Hvalid=>//.
+    apply auth_valid_discrete_2 in Hvalid as [[af Compose%leibniz_equiv_iff] Valid].
+    destruct agy as [y|].
+    - iDestruct "Hauth" as "[? ?]". iFrame.
+      iPureIntro. apply f_equal.
+      eapply (map_agree_eq _ _ _ m)=>//.
+    - iAssert (✓ m)%I as "H"=>//. rewrite (gmap_validI m).
+      iDestruct ("H" $! hd) as "%".
+      exfalso. subst. rewrite H0 in H1.
+      by destruct H1 as [? ?].
+  Qed.
+  
+  Lemma evmap_frag_agree_split γm p q1 q2 (a1 a2: A):
+    own γm (◯ {[p := (q1, DecAgree a1)]}) ★
+    own γm (◯ {[p := (q2, DecAgree a2)]})
+    ⊢ (a1 = a2).
+  Proof.
+    iIntros "[Ho Ho']".
+    destruct (decide (a1 = a2)) as [->|Hneq].
+    - by iFrame.
+    - iCombine "Ho" "Ho'" as "Ho".
+      rewrite -(@auth_frag_op (evmapR K A unitR) {[p := (q1, DecAgree a1)]} {[p := (q2, DecAgree a2)]}).
+      iDestruct (own_valid with "Ho") as %Hvalid.
+      exfalso. 
+      rewrite op_singleton in Hvalid.
+      apply auth_valid_discrete in Hvalid. simpl in Hvalid.
+      apply singleton_valid in Hvalid.
+      destruct Hvalid as [_ Hvalid].
+      apply dec_agree_op_inv in Hvalid. inversion Hvalid. subst. auto.
+  Qed.
+End evmapR.
+
